\documentclass{article}

\usepackage{minted}
\usepackage{graphicx}
\usepackage{geometry}
\usepackage{amsmath}
\usepackage[final]{pdfpages} 


\geometry{hmargin=0.5cm,vmargin=0.5cm}
\newcommand{\g}[2]{g_{#1}^{#2}}
%\newcommand{\g}[2]{g(#1, #2)}


\begin{document}


\begin{align*}
\g{s}{1} &= z ( p  \g{s+1}{1} + q \g{s-1}{-1} ) \\
\g{s+1}{1} &= \frac{1}{z p} \g{s}{1} - \frac{q}{p} \g{s-1}{-1} 
\end{align*}

\begin{align*}
\g{s}{-1} &= z ( q \g{s+1}{1} + p \g{s-1}{-1} ) \\
\g{s+1}{-1} &= z ( q \g{s+2}{1} + p \g{s}{-1} ) \\
\g{s+1}{-1} &= z ( \frac{q}{z p} \g{s+1}{1} - \frac{q^2}{p} \g{s}{-1} + p \g{s}{-1} ) \\
\g{s+1}{-1} &= z ( \frac{q}{z p} \g{s+1}{1} + (p - \frac{q^2}{p}) \g{s}{-1}  ) \\
\g{s+1}{-1} &=  \frac{q}{p} \g{s+1}{1} + z(p - \frac{q^2}{p}) \g{s}{-1}  \\
\g{s+1}{-1} &=  \frac{q}{p} ( \frac{1}{z p} \g{s}{1} - \frac{q}{p} \g{s-1}{-1} ) + z(p - \frac{q^2}{p}) \g{s}{-1}  \\
\g{s+1}{-1} &=  \frac{q}{z p^2} \g{s}{1} + \left( z(p - \frac{q^2}{p}) - ( \frac{q}{p} )^2 \right) \g{s}{-1}  
\end{align*}

\begin{align*}
G_{s+1} = 
\begin{pmatrix} 
\g{s+1}{1} \\ \g{s+1}{-1} \\ \g{s}{1} \\ \g{s}{-1} 
\end{pmatrix}
&= 
\begin{pmatrix} 
\frac{1}{z p} & 0 &  0 &  \frac{q}{p} \\
\frac{q}{p} & z(p - \frac{q^2}{p}) - ( \frac{q}{p} )^2 &  0 & 0\\
1 & 0 &  0 & 0\\
0 & 1 &  0 & 0
\end{pmatrix}
.
\begin{pmatrix} 
\g{s}{1} \\ \g{s}{-1} \\ \g{s-1}{1} \\ \g{s-1}{-1} 
\end{pmatrix} \\
&= 
A(z). G_s
\end{align*}


\end{document}
